messageInvariantPrototypes/clientServer/centralized/spec.dfy
@@ -10,8 +10,8 @@ module Obligations {
     requires c.WF()
     requires v.WF(c)
   {
-  forall cidx:nat | c.ValidClientIdx(cidx)
-    :: SafetySingleClient(v.hosts[cidx].client)
+    forall cidx:nat | c.ValidClientIdx(cidx)
+      :: SafetySingleClient(v.hosts[cidx].client)
   }
 
   ghost predicate SafetySingleClient(v: ClientHost.Variables) {
